theories/iris_fundamental.v
@@ -16,7 +16,11 @@ Section fundamental.
   Import DummyHosts. (* placeholder *)
 
   Context `{!wfuncG Σ, !wtabG Σ, !wmemG Σ, !wmemsizeG Σ, !wglobG Σ, !wframeG Σ, HWP: host_program_logic, !logrel_na_invs Σ}.
-
+  
+  (* --------------------------------------------------------------------------------------- *)
+  (* ------------------------------ HELPER TACTICS AND LEMMAS ------------------------------ *)
+  (* --------------------------------------------------------------------------------------- *)
+  
   Ltac take_drop_app_rewrite n :=
     match goal with
     | |- context [ WP ?e @ _; _ CTX _; _ {{ _ }} %I ] =>
@@ -37,110 +41,158 @@ Section fundamental.
     | |- context [ WP _ ++ ?e @ _; _ {{ _ }} %I ] =>
         rewrite -(list.take_drop (length e - m) e);simpl take; simpl drop
     end.
+  (* Helper lemmas and tactics for necessary list manipulations for expressions *)
+  Lemma iRewrite_nil_l (s : stuckness) (E : coPset) (Φ : val -> iProp Σ) (e : iris.expr) :
+    (WP [] ++ e @ s; E {{ Φ }} ⊢ WP e @ s; E {{ Φ }}).
+  Proof. rewrite app_nil_l. auto. Qed.
+  Lemma iRewrite_nil_r (s : stuckness) (E : coPset) (Φ : val -> iProp Σ) (e : iris.expr) :
+    (WP e ++ [] @ s; E {{ Φ }} ⊢ WP e @ s; E {{ Φ }}).
+  Proof. rewrite app_nil_r. auto. Qed.
+  Lemma iRewrite_nil_l_ctx (s : stuckness) (E : coPset) (Φ : val -> iProp Σ) (e : iris.expr) i lh :
+    (WP [] ++ e @ s; E CTX i; lh {{ Φ }} ⊢ WP e @ s; E CTX i; lh {{ Φ }}).
+  Proof. rewrite app_nil_l. auto. Qed.
+  Lemma iRewrite_nil_r_ctx (s : stuckness) (E : coPset) (Φ : val -> iProp Σ) (e : iris.expr) i lh :
+    (WP e ++ [] @ s; E CTX i; lh {{ Φ }} ⊢ WP e @ s; E CTX i; lh {{ Φ }}).
+  Proof. rewrite app_nil_r. auto. Qed.
+
+  Lemma wp_wand_ctx s E e Φ Ψ i lh :
+    WP e @ s; E CTX i; lh {{ Φ }} -∗ (∀ v, Φ v -∗ Ψ v) -∗ WP e @ s; E CTX i; lh {{ Ψ }}.
+  Proof.
+    iIntros "Hwp H". iIntros (LI HLI).
+    iSpecialize ("Hwp" $! LI HLI).
+    iApply (wp_wand with "Hwp"). auto.
+  Qed.
 
   Lemma interp_value_type_of v : (⊢ interp_value (Σ:=Σ) (typeof v) v)%I.
   Proof.
     unfold interp_value.
     destruct v;simpl;eauto.
   Qed.
+
+  Lemma const_list_of_val vs :
+    const_list (of_val (immV vs)).
+  Proof.
+    induction vs;auto. Qed.
+
+
+
+
+  (* --------------------------------------------------------------------------------------- *)
+  (* -------------------------------------- EXPRESSIONS ------------------------------------ *)
+  (* --------------------------------------------------------------------------------------- *)
+
+  Lemma typing_const C v : ⊢ semantic_typing (HWP:=HWP) C (to_e_list [BI_const v]) (Tf [] [typeof v]).
+  Proof.
+    unfold semantic_typing, interp_expression.
+    iIntros (i lh f vs).
+    iIntros "#Hi %Hlh #Hv Hf".
+    iDestruct "Hf" as (locs Heq) "[#Hlocs Hf]".
+    iDestruct "Hv" as "[-> | Hv]".
+    { take_drop_app_rewrite_twice 0 1.
+      iApply (wp_wand_r _ _ _ (λ vs, interp_val [typeof v] vs ∗  ↪[frame]f)%I). iSplitL.
+      { iApply (wp_trap with "[] [$]");auto. by iLeft. }
+      iIntros (v0) "[? ?]". iFrame. iExists _. iFrame. }
+    { iDestruct "Hv" as (ws ->) "Hv".
+      iDestruct (big_sepL2_nil_inv_r with "Hv") as %->.
+      iApply (wp_wand_r _ _ _ (λ vs, interp_val [typeof v] vs ∗  ↪[frame]f)%I). iSplitL.
+      { rewrite app_nil_l.
+        iApply wp_value;[by instantiate (1:= immV [_])|].
+        iFrame. iRight. iExists _. iSplit;eauto.
+        iSimpl; iSplit =>//. iApply interp_value_type_of. }
+      iIntros (v0) "[? ?]". iFrame. iExists _. iFrame. 
+    }
+  Qed.
+
+  Lemma typing_loop C es tn tm : (⊢ semantic_typing (HWP:=HWP) (upd_label C ([tn] ++ tc_label C)%list) (to_e_list es) (Tf tn tm)) ->
+                                 ⊢ semantic_typing (HWP:=HWP) C (to_e_list [BI_loop (Tf tn tm) es]) (Tf tn tm).
+  Proof.
+    intros IHbe_typing.
+    unfold semantic_typing, interp_expression.
+    iIntros (i lh f vs).
+    iIntros "#Hi %Hlh #Hv Hf".
+    iDestruct "Hv" as "[-> | Hv]".
+    { iDestruct "Hf" as (locs Heq) "[#Hlocs Hf]". 
+      take_drop_app_rewrite_twice 0 1.
+      iApply (wp_wand_r _ _ _ (λ vs, interp_val tm vs ∗  ↪[frame]f)%I). iSplitL.
+      { iApply (wp_trap with "[] [$]");auto. by iLeft. }
+      iIntros (v0) "[? ?]". iFrame. iExists _. iFrame. }
+    iDestruct "Hv" as (ws ->) "Hv".
+    iDestruct (big_sepL2_length with "Hv") as %Hlen.
+    iDestruct "Hf" as (locs Heq) "[#Hlocs Hf]".
+    iApply (wp_loop with "Hf");eauto.
+    { apply v_to_e_is_const_list. }
+    { rewrite fmap_length //. }
+    iNext. iIntros "Hf".
+    iDestruct (IHbe_typing with "[] [] []") as "HH";try by (destruct C,i;eauto).
+    { unfold interp_ctx. simpl. instantiate (1:=LH_rec (of_val (immV ws)) (length tn) _ lh _).
+      iPureIntro. destruct Hlh as [Hbase Hlenh]. auto. }
+    { instantiate (1:=immV ws). iRight. eauto. }
+    iAssert (↪[frame]f -∗ WP of_val (immV ws) ++ to_e_list es
+                {{ vs, interp_val tm vs ∗ (∃ f0 : leibnizO frame,  ↪[frame]f0) }})%I as "Hcont".
+    { iIntros "Hf". iApply "HH". iFrame. iExists _. eauto. }
+    iApply wp_wasm_empty_ctx.
+    iApply wp_label_push_nil.
+    iApply iRewrite_nil_r_ctx.
+    iApply wp_seq_can_trap_ctx. iFrame "∗ #". 
+    iSplitR.
+    { iIntros "Hcontr".
+        iDestruct "Hcontr" as (ws0 Hcontr) "_". done. }
+    iSplitR.
+    { iLeft. auto. }
+    iIntros (w f0) "Hres".
+    iDestruct "Hres" as "[Hw Hf]".
+    iDestruct "Hw" as (vs ->) "Hvs".
+    rewrite app_nil_r. simpl push_base.
+    iApply (wp_wand_ctx with "[-]").
+    { iApply (wp_val_return with "Hf").
+      { apply const_list_of_val. }
+      iIntros "Hf". iFrame.
+      instantiate (1:=interp_val tm).
+      instantiate (2:=[]). instantiate (1:=[]).
+      iApply wp_value;[by rewrite app_nil_l app_nil_r|iRight;eauto]. }
+    { iIntros (v) "[Hw Hf]". iFrame. eauto. }
+  Qed.
     
+    
+  (* --------------------------------------------------------------------------------------- *)
+  (* ------------------------------- FTLR: simple typing ----------------------------------- *)
+  (* --------------------------------------------------------------------------------------- *)
+  
   Theorem be_fundamental C es τ : be_typing C es τ -> ⊢ semantic_typing (HWP:=HWP) C (to_e_list es) τ.
   Proof.
     induction 1.
-    
-    {
-      unfold semantic_typing, interp_expression.
-      iIntros (i lh f vs).
-      destruct C,i.
-      iIntros "(#Hi & Hf & %Hlh) #Hv".
-      iDestruct "Hf" as (locs Heq) "[#Hlocs Hf]".
-      iDestruct "Hv" as "[-> | Hv]".
-      { take_drop_app_rewrite_twice 0 1.
-        iApply (wp_wand_r _ _ _ (λ vs, interp_val [typeof v] vs ∗  ↪[frame]f)%I). iSplitL.
-        { iApply (wp_trap with "[] [$]");auto. by iLeft. }
-        iIntros (v0) "[? ?]". iFrame. iExists _. iFrame. }
-      { iDestruct "Hv" as (ws ->) "Hv".
-        iDestruct (big_sepL2_nil_inv_r with "Hv") as %->.
-        iApply (wp_wand_r _ _ _ (λ vs, interp_val [typeof v] vs ∗  ↪[frame]f)%I). iSplitL.
-        { rewrite app_nil_l.
-          iApply wp_value;[by instantiate (1:= immV [_])|].
-          iFrame. iRight. iExists _. iSplit;eauto.
-          iSimpl; iSplit =>//. iApply interp_value_type_of. }
-        iIntros (v0) "[? ?]". iFrame. iExists _. iFrame. 
-      }
-    }
-
-
-    12: {
-      unfold semantic_typing, interp_expression.
-      iIntros (i lh f vs).
-      destruct C,i.
-      set (C := {|
-                 tc_types_t := tc_types_t;
-                 tc_func_t := tc_func_t;
-                 tc_global := tc_global;
-                 tc_table := tc_table;
-                 tc_memory := tc_memory;
-                 tc_local := tc_local;
-                 tc_label := tc_label;
-                 tc_return := tc_return
-               |}
-          ).
-      set (i := {|
-                 inst_types := inst_types;
-                 inst_funcs := inst_funcs;
-                 inst_tab := inst_tab;
-                 inst_memory := inst_memory;
-                 inst_globs := inst_globs
-               |}).
-      iIntros "(#Hi & Hf & %Hlh) #Hv".
-      iDestruct "Hv" as "[-> | Hv]".
-      { iDestruct "Hf" as (locs Heq) "[#Hlocs Hf]". 
-        take_drop_app_rewrite_twice 0 1.
-        iApply (wp_wand_r _ _ _ (λ vs, interp_val tm vs ∗  ↪[frame]f)%I). iSplitL.
-        { iApply (wp_trap with "[] [$]");auto. by iLeft. }
-        iIntros (v0) "[? ?]". iFrame. iExists _. iFrame. }
-      iDestruct "Hv" as (ws ->) "Hv".
-      iDestruct (big_sepL2_length with "Hv") as %Hlen.
-      iDestruct "Hf" as (locs Heq) "[#Hlocs Hf]".
-      iApply (wp_loop with "Hf");eauto.
-      { apply v_to_e_is_const_list. }
-      { rewrite fmap_length //. }
-      iNext. iIntros "Hf".
-      iDestruct (IHbe_typing with "[Hf] []") as "HH".
-      { iFrame "# ∗". unfold interp_ctx. simpl. instantiate (1:=LH_rec (of_val (immV ws)) (length tn) _ lh _).
-        iSplit;[iExists _;eauto|].
-        iPureIntro. destruct Hlh as [Hbase Hlenh]. auto. }
-      { instantiate (1:=immV ws). iRight. eauto. }
-      iApply wp_wasm_empty_ctx.
-      iApply wp_label_push_nil. iSimpl.
-      unfold interp_expression,interp_val.
-      iAssert (WP of_val (immV ws) ++ to_e_list es
-                  {{ vs, ⌜vs = trapV⌝ ∗ (∃ f0 : leibnizO frame,  ↪[frame]f0) }} ∨
-              WP of_val (immV ws) ++ to_e_list es
-                 {{ vs, (∃ ws0 : seq.seq (leibnizO value), ⌜vs = immV ws0⌝ ∗ ([∗ list] w;τ ∈ ws0;tm, interp_value τ w))
-                          ∗ (∃ f0 : leibnizO frame,  ↪[frame]f0) }})%I with "[HH]" as "HHH".
-      { }
-
-      
-      iApply wp_seq_ctx.
-
-      iDestruct "HH" as (f0) "HH". iExists f0.
-      
-
-
-      
-      iDestruct (IHbe_typing with "[Hf] []") as "HH".
-      { iFrame "# ∗". unfold interp_ctx. simpl. instantiate (1:=LH_rec (of_val (immV ws)) (length tn) _ lh _).
-        iPureIntro. destruct Hlh as [Hbase Hlen]. auto. }
-      { instantiate (1:=immV ws). iRight. eauto. }
-      iDestruct "HH" as (f0) "HH". iExists f0.
-      iDestruct (big_sepL2_length with "Hv") as %Hlen.
-      iApply wp_loop;eauto.
-      { apply v_to_e_is_const_list. }
-      { rewrite fmap_length //. }
-      { eauto. } apply const_list_of_val.
-     
-
+    { apply typing_const. }
+    { admit. }
+    { admit. }
+    { admit. }
+    { admit. }
+    { admit. }
+    { admit. }
+    { admit. }
+    { admit. }
+    { admit. }
+    { admit. }
+    { admit. }
+    { by apply typing_loop. }
+    { admit. }
+    { admit. }
+    { admit. }
+    { admit. }
+    { admit. }
+    { admit. }
+    { admit. }
+    { admit. }
+    { admit. }
+    { admit. }
+    { admit. }
+    { admit. }
+    { admit. }
+    { admit. }
+    { admit. }
+    { admit. }
+    { admit. }
+    { admit. }
+    { admit. }
+  Admitted.
 
 End fundamental.
