theories/iris_rules.v
@@ -5,7 +5,13 @@ From iris.proofmode Require Import base tactics classes.
 From iris.base_logic Require Export gen_heap ghost_map proph_map.
 From iris.base_logic.lib Require Export fancy_updates.
 Require Export iris iris_locations iris_properties iris_atomicity stdpp_aux.
-Require Export iris_rules_structural iris_rules_pure iris_rules_control iris_rules_resources iris_rules_calls iris_rules_trap.
+Require Export iris_rules_structural
+        iris_rules_pure
+        iris_rules_control
+        iris_rules_resources
+        iris_rules_calls
+        iris_rules_trap
+        iris_rules_structural_with_trap.
 Require Export datatypes host operations properties opsem.
 
 Context `{!wfuncG Σ, !wtabG Σ, !wmemG Σ, !wmemsizeG Σ, !wglobG Σ, !wframeG Σ}.
